```Haskell
class Monoid m where
    mempty  :: m
    mappend :: m -> m -> m
```
```tut:silent
trait Monoid[M] {
  def mempty: M
  def mappend(m1: M, m2: M): M
}
```
................
```Haskell
instance Monoid [a] where
    mempty = []
    mappend = (++)
```
```tut:silent
object Monoid {
  implicit def listMonoid[A]: Monoid[List[A]] = new Monoid[List[A]] {
    def mempty: List[A] = List()
    def mappend(m1: List[A], m2: List[A]): List[A] = m1 ++ m2
  }
}
```
................
```Haskell
2 * 3 = 6
[2] ++ [3] = [2, 3] // not the same as [6]
```
```tut:silent
2 * 3 == 6
List(2) ++ List(3) == List(2, 3)
```
................
```Haskell
h (a * b) = h a * h b
```
```scala
h(a * b) == h(a) * h(b)
```
................
```Haskell
[2] ++ [3] = [2, 3]
```
```tut:silent
List(2) ++ List(3) == List(2, 3)
```
................
```Haskell
2 * 3 = 6
```
```tut:silent
2 * 3 == 6
```
................
```Haskell
p :: x -> U m
```
```scala
val p: X => U[M]
```
................
```Haskell
q :: x -> U n
```
```scala
val q: X => U[N]
```
................
```Haskell
h :: m -> n
```
```scala
val h: M => N
```
................
```Haskell
q = U h . p
```
```scala
val q = uh compose p
```
................
```Haskell
h a * h e = h (a * e) = h a
```
```scala
h(a) * h(e) == h(a * e) == h(a)
```