```tut:invisible
// some preparation to make tut happy
trait Functor[F[_]] {
  def fmap[A, B](f: A => B)(fa: F[A]): F[B]
}
```
................
```Haskell
μ :: m × m -> m
η :: 1 -> m
```
```scala
def μ[M]: M × M => M
def η[M]: 1 => M
```
................
```Haskell
F a -> a
```
```scala
F[A] => A
```
................
```Haskell
type Algebra f a = f a -> a
```
```tut:silent
type Algebra[F[_], A] = F[A] => A
```
................
```Haskell
data MonF a = MEmpty | MAppend a a
```
```tut:silent
sealed trait MonF[+A] extends
    Product with Serializable
case object MEmpty extends MonF[Nothing]
final case class MAppend[A](
    m: A, n: A) extends MonF[A]
```
................
```Haskell
data RingF a = RZero
             | ROne
             | RAdd a a
             | RMul a a
             | RNeg a
```
```tut:silent
sealed trait RingF[+A] extends
    Product with Serializable
case object RZero extends RingF[Nothing]
case object ROne extends RingF[Nothing]
final case class RAdd[A](
    m: A, n: A) extends RingF[A]
final case class RMul[A](
    m: A, n: A) extends RingF[A]
final case class RNeg[A](
    n: A) extends RingF[A]
```
................
```Haskell
evalZ :: Algebra RingF Integer
evalZ RZero      = 0
evalZ ROne       = 1
evalZ (RAdd m n) = m + n
evalZ (RMul m n) = m * n
evalZ (RNeg n)   = -n
```
```tut:silent
def evalZ: Algebra[RingF, Int] = {
  case RZero => 0
  case ROne => 1
  case RAdd(m, n) => m + n
  case RMul(m, n) => m * n
  case RNeg(n) => -n
}
```
................
```Haskell
data Expr = RZero
          | ROne
          | RAdd Expr Expr
          | RMul Expr Expr
          | RNeg Expr
```
```tut:silent
sealed trait Expr extends
    Product with Serializable
case object RZero extends Expr
case object ROne extends Expr
final case class RAdd(
    e1: Expr, e2: Expr) extends Expr
final case class RMul(
    e1: Expr, e2: Expr) extends Expr
final case class RNeg(
    e: Expr) extends Expr
```
................
```Haskell
evalZ :: Expr -> Integer
evalZ RZero        = 0
evalZ ROne         = 1
evalZ (RAdd e1 e2) = evalZ e1 + evalZ e2
evalZ (RMul e1 e2) = evalZ e1 * evalZ e2
evalZ (RNeg e)     = -(evalZ e)
```
```tut:silent
def evalZ: Expr => Int = {
  case RZero => 0
  case ROne => 1
  case RAdd(e1, e2) => evalZ(e1) + evalZ(e2)
  case RMul(e1, e2) => evalZ(e1) * evalZ(e2)
  case RNeg(e) => -evalZ(e)
}
```
................
```Haskell
type RingF1 a = RingF (RingF a)
```
```tut:silent
type RingF1[A] = RingF[RingF[A]]
```
................
```Haskell
type RingF2 a = RingF (RingF (RingF a))
```
```tut:silent
type RingF2[A] = RingF[RingF[RingF[A]]]
```
................
```Haskell
type RingF2 a = RingF (RingF1 a)
```
```tut:silent
type RingF2[A] = RingF[RingF1[A]]
```
................
```Haskell
type RingFn+1 a = RingF (RingFn a)
```
```scala
type `RingFn+1`[A] = RingF[RingFn[A]]
```
................
```Haskell
Fix f = f (Fix f)
```
```scala
Fix[F] == F[Fix[F]]
```
................
```Haskell
newtype Fix f = Fix (f (Fix f))
```
```tut:silent
case class Fix[F[_]](x: F[Fix[F]])
```
................
```Haskell
newtype Fix f = In (f (Fix f))
```
```scala
sealed trait Fix[F[_]] extends
    Product with Serializable
final case class In[F[_]](f: F[Fix[F]])
```
................
```Haskell
Fix :: f (Fix f) -> Fix f
```
```scala
object Fix {
  def apply[F[_]](f: F[Fix[F]]): Fix[F] =
    new Fix(f)
}
```
................
```Haskell
unFix :: Fix f -> f (Fix f)
unFix (Fix x) = x
```
```tut:silent
def unFix[F[_]]: Fix[F] => F[Fix[F]] = {
  case Fix(x) => x
}
```
................
```Haskell
zero :: 1 -> N
succ :: N -> N
```
```scala
def zero: 1 => N
def succ: N => N
```
................
```Haskell
data NatF a = ZeroF | SuccF a
```
```tut:silent
sealed trait NatF[+A] extends
    Product with Serializable
case object ZeroF extends NatF[Nothing]
final case class SuccF[A](
    a: A) extends NatF[A]
```
................
```Haskell
data Nat = Zero | Succ Nat
```
```tut:silent
sealed trait Nat extends
    Product with Serializable
case object Zero extends Nat
final case class Succ(n: Nat) extends Nat
```
................
```Haskell
cata :: Functor f => (f a -> a) -> Fix f -> a
cata alg = alg . fmap (cata alg) . unFix
```
```tut:silent
def cata[F[_], A](alg: F[A] => A)
    (implicit F: Functor[F]): Fix[F] => A =
  alg.compose(
    F.fmap(cata(alg)) _ compose unFix)
```
................
```Haskell
data NatF a = ZeroF | SuccF a
```
```tut:silent
sealed trait NatF[+A] extends
    Product with Serializable
case object ZeroF extends NatF[Nothing]
final case class SuccF[A](
    a: A) extends NatF[A]
```
................
```Haskell
fib :: NatF (Int, Int) -> (Int, Int)
fib ZeroF = (1, 1)
fib (SuccF (m, n)) = (n, m + n)
```
```tut:silent
def fib: NatF[(Int, Int)] => (Int, Int) = {
  case ZeroF => (1, 1)
  case SuccF((m, n)) => (n, m + n)
}
```
................
```Haskell
data ListF e a = NilF | ConsF e a
```
```tut:silent
sealed trait ListF[+E, +A] extends
    Product with Serializable
case object NilF extends
    ListF[Nothing, Nothing]
final case class ConsF[E, A](
    h: E, t: A) extends ListF[E, A]
```
................
```Haskell
data List e = Nil | Cons e (List e)
```
```tut:silent
sealed trait List[+E] extends
    Product with Serializable
case object Nil extends List[Nothing]
final case class Cons[E](
    h: E, t: List[E]) extends List[E]
```
................
```Haskell
lenAlg :: ListF e Int -> Int
lenAlg (ConsF e n) = n + 1
lenAlg NilF = 0
```
```tut:silent
def lenAlg[E]: ListF[E, Int] => Int = {
  case ConsF(e, n) => n + 1
  case NilF => 0
}
```
................
```Haskell
length = foldr (\e n -> n + 1) 0
```
```tut:silent
import scala.collection.immutable.List
def length[E](l: List[E]): Int =
  l.foldRight(0)((e, n) => n + 1)
```
................
```Haskell
sumAlg :: ListF Double Double -> Double
sumAlg (ConsF e s) = e + s
sumAlg NilF = 0.0
```
```tut:silent
def sumAlg
    : ListF[Double, Double] => Double = {
  case ConsF(e, s) => e + s
  case NilF => 0.0
}
```
................
```Haskell
sum = foldr (\e s -> e + s) 0.0
```
```tut:silent
import scala.collection.immutable.List
def sum(l: List[Double]): Double =
  l.foldRight(0.0)((e, s) => e + s)
```
................
```Haskell
a -> F a
```
```scala
A => F[A]
```
................
```Haskell
ana :: Functor f => (a -> f a) -> a -> Fix f
ana coalg = Fix . fmap (ana coalg) . coalg
```
```tut:silent
def ana[F[_], A](coalg: A => F[A])
    (implicit F: Functor[F]): A => Fix[F] =
  (Fix.apply[F] _).compose(
    F.fmap(ana(coalg)) _ compose coalg)
```
................
```Haskell
data StreamF e a = StreamF e a
  deriving Functor
```
```tut:silent
final case class StreamF[E, A](h: E, t: A)
implicit def streamFFunctor[E] =
  new Functor[({type T[A] = StreamF[E, A]})#T] {
    def fmap[A, B](f: A => B)
        (fa: StreamF[E, A])
        : StreamF[E, B] = ???
  }
```
................
```Haskell
data Stream e = Stream e (Stream e)
```
```tut:silent
final
case class Stream[E](h: E, t: Stream[E])
```
................
```Haskell
era :: [Int] -> StreamF Int [Int]
era (p : ns) = StreamF p (filter (notdiv p) ns)
    where notdiv p n = n `mod` p /= 0
```
```tut:silent
import scala.collection.immutable.List
def era: List[Int]
    => StreamF[Int, List[Int]] = {
  case p :: ns =>
    def notdiv(p: Int)(n: Int): Boolean =
      n % p != 0
    StreamF(p, ns.filter(notdiv(p)))
}
```
................
```Haskell
primes = ana era [2..]
```
```tut:silent
// just, imagine that the list is infinite
def primes =
  ana(era)(streamFFunctor)((1 to 10).toList)
```
................
```Haskell
toListC :: Fix (StreamF e) -> [e]
toListC = cata al
   where al :: StreamF e [e] -> [e]
         al (StreamF e a) = e : a
```
```tut:silent
def toListC[E]
    : Fix[({type T[A] = StreamF[E, A]})#T]
    => List[E] = {
  def al: StreamF[E, List[E]] => List[E] = {
    case StreamF(e, a) => e :: a
  }
  cata[
    ({type T[A] = StreamF[E, A]})#T, List[E]
  ](al)
}

/* type lambda with Kind Projector plugin:
   Fix[StreamF[E, ?]] */
```
................
```Haskell
unfoldr :: (b -> Maybe (a, b)) -> b -> [a]
```
```scala
def unfoldr[A, B]
    : (B => Option[(A, B)]) => B => List[A]
```
................
```Haskell
set :: a -> s -> a
get :: a -> s
```
```scala
def set[A, S]: A => S => A
def get[A, S]: A => S
```
................
```Haskell
a -> (s, s -> a)
```
```scala
A => ((S, S => A))
```
................
```Haskell
a -> Store s a
```
```scala
A => Store[S, A]
```
................
```Haskell
data Store s a = Store (s -> a) s
```
```tut:silent
case class Store[S, A](run: S => A, s: S)
```
